Separated ProcDecInl

examples/ProcDecInv.v
@@ -3,7 +3,7 @@ Require Import Lib.CommonTactics Lib.ilist Lib.Word.
 Require Import Lib.Struct Lib.StringBound Lib.FMap Lib.StringEq.
 Require Import Lts.Syntax Lts.Semantics Lts.Equiv Lts.Refinement Lts.Renaming Lts.Wf.
 Require Import Lts.Renaming Lts.Specialize Lts.Inline Lts.InlineFacts_2 Lts.DecompositionZero.
-Require Import Ex.SC Ex.Fifo Ex.MemAtomic Ex.ProcDec.
+Require Import Ex.SC Ex.Fifo Ex.MemAtomic Ex.ProcDec Ex.ProcDecInl.
 Require Import Eqdep.
 
 Set Implicit Arguments.
@@ -42,11 +42,54 @@ Ltac kexistv k v m t :=
   refine (exists v: fullType type (SyntaxKind t),
              M.find k m = Some (existT _ _ v) /\ _).
 
+Ltac simpl_find :=
+  repeat
+    match goal with
+    | [H1: M.find ?k ?m = _, H2: M.find ?k ?m = _ |- _] =>
+      rewrite H1 in H2
+    | [H: Some _ = Some _ |- _] => inv H
+    end; destruct_existT.
+
+Ltac invReify :=
+  repeat (eexists; split; [findReify; simpl; eauto|]).
+
+Ltac inv_red :=
+  repeat autounfold with InvDefs in *; dest; simpl_find;
+  repeat
+    (match goal with
+     (* Logic *)
+     | [ |- ~ _ ] => intro
+     | [H: _ \/ _ |- _] => destruct H
+     | [ |- _ /\ _ ] => split
+     | [H: ?t = ?t |- _] => clear H
+     (* Reducing boolean conditions *)
+     | [H: false = true |- _] => inversion H
+     | [H: true = false |- _] => inversion H
+     | [H: negb _ = true |- _] => apply negb_true_iff in H; subst
+     | [H: negb _ = false |- _] => apply negb_false_iff in H; subst
+     end; dest; try subst).
+
+Ltac inv_solve :=
+  abstract (
+      inv_red;
+      repeat
+        (try
+           match goal with
+           (* Destruction *)
+           | [H: context [weq ?w1 ?w2] |- _] => destruct (weq w1 w2)
+           | [ |- context [weq ?w1 ?w2] ] => destruct (weq w1 w2)
+           end;
+         try subst;
+         intuition idtac)
+    ).
+
 Section Invariants.
   Variables addrSize fifoSize valSize rfIdx: nat.
 
   Variable dec: DecT 2 addrSize valSize rfIdx.
   Variable exec: ExecT 2 addrSize valSize rfIdx.
+
+  Definition pdecInl := pdecInl fifoSize dec exec.
 
   Definition procDec_inv_0 (o: RegsT): Prop.
   Proof.
@@ -75,9 +118,7 @@ Section Invariants.
     fifoEmpty = true /\ fifoEnqP = fifoDeqP.
   
   Definition fifo_not_empty_inv (fifoEmpty: bool) (fifoEnqP fifoDeqP: type (Bit fifoSize)): Prop :=
-    fifoEmpty = false /\
-    ((fifoDeqP <> ^~ $1 /\ fifoEnqP = fifoDeqP ^+ $1) \/
-     (fifoDeqP = ^~ $1 /\ fifoEnqP = $0)).
+    fifoEmpty = false /\ fifoEnqP = fifoDeqP ^+ $1.
 
   Hint Unfold xor3 fifo_empty_inv fifo_not_empty_inv: InvDefs.
 
@@ -96,57 +137,70 @@ Section Invariants.
     - exact (v = true /\ fifo_empty_inv v0 v1 v2 /\ fifo_not_empty_inv v3 v4 v5).
   Defined.
 
-  Definition pdec := pdecf fifoSize dec exec.
-  Hint Unfold pdec: ModuleDefs. (* for kinline_compute *)
-
-  Definition pdecInl: Modules * bool.
+  Definition procDec_inv_2 (o: RegsT): Prop.
   Proof.
-    remember (inlineF pdec) as inlined.
-    kinline_compute_in Heqinlined.
-    match goal with
-    | [H: inlined = ?m |- _] =>
-      exact m
-    end.
+    kexistv "pc"%string pcv o (Bit addrSize).
+    kexistv "rf"%string rfv o (Vector (Bit valSize) rfIdx).
+    kexistv "Ins.empty"%string iev o Bool.
+    kexistv "Ins.elt"%string ieltv o (Vector (memAtomK addrSize valSize) fifoSize).
+    kexistv "Ins.deqP"%string ideqP o (Bit fifoSize).
+    refine (if v1 then True else _).
+    exact (dec _ v0 v ``"opcode" = v2 v3 ``"type").
   Defined.
 
-  Lemma pdecInl_equal: pdecInl = inlineF pdec.
+  Lemma procDec_inv_0_ok':
+    forall init n ll,
+      init = initRegs (getRegInits (fst pdecInl)) ->
+      Multistep (fst pdecInl) init n ll ->
+      procDec_inv_0 n.
   Proof.
     admit.
-    (* kinline_compute. *)
-    (* reflexivity. *)
+    (* induction 2. *)
+
+    (* - repeat subst. *)
+    (*   simpl; unfold procDec_inv_0. *)
+    (*   invReify; auto. *)
+
+    (* - specialize (IHMultistep H); clear -IHMultistep HStep. *)
+    (*   apply step_no_defs_substep in HStep; [|reflexivity]. *)
+    (*   destruct HStep as [ul [calls ?]]; dest; subst. *)
+    (*   inv H0; try (mred; fail); [|inv HIn]. *)
+    (*   CommonTactics.dest_in. *)
+
+    (*   + inv H; invertActionRep. *)
+    (*     unfold procDec_inv_0 in *; dest. *)
+    (*     invReify; simpl_find; auto. *)
+    (*   + inv H0; invertActionRep. *)
+    (*     unfold procDec_inv_0 in *; dest. *)
+    (*     invReify; simpl_find; auto. *)
+    (*   + inv H; invertActionRep. *)
+    (*     unfold procDec_inv_0 in *; dest. *)
+    (*     invReify; simpl_find; auto. *)
+    (*   + inv H0; invertActionRep. *)
+    (*     unfold procDec_inv_0 in *; dest. *)
+    (*     invReify; simpl_find; auto. *)
+    (*   + inv H; invertActionRep. *)
+    (*     unfold procDec_inv_0 in *; dest. *)
+    (*     invReify; simpl_find; auto. *)
+    (*   + inv H0; invertActionRep. *)
+    (*     unfold procDec_inv_0 in *; dest. *)
+    (*     invReify; simpl_find; auto. *)
+    (*   + inv H; invertActionRep. *)
+    (*     unfold procDec_inv_0 in *; dest. *)
+    (*     invReify; simpl_find; auto. *)
+    (*   + inv H0; invertActionRep. *)
+    (*     unfold procDec_inv_0 in *; dest. *)
+    (*     invReify; simpl_find; auto. *)
   Qed.
 
-  Ltac simpl_find :=
-    repeat
-      match goal with
-      | [H1: M.find ?k ?m = _, H2: M.find ?k ?m = _ |- _] =>
-        rewrite H1 in H2
-      | [H: Some _ = Some _ |- _] => inv H
-      end; destruct_existT.
-
-  Ltac invReify :=
-    repeat (eexists; split; [findReify; simpl; eauto|]).
-
-  Ltac inv_solve :=
-    abstract (
-        repeat autounfold with InvDefs in *;
-        repeat
-          (match goal with
-           (* Logic *)
-           | [ |- ~ _ ] => intro
-           | [H: _ \/ _ |- _] => destruct H
-           | [ |- _ /\ _ ] => split
-           | [H: ?t = ?t |- _] => clear H
-           (* Reducing boolean conditions *)
-           | [H: false = true |- _] => inversion H
-           | [H: true = false |- _] => inversion H
-           | [H: negb _ = true |- _] => apply negb_true_iff in H; subst
-           | [H: negb _ = false |- _] => apply negb_false_iff in H; subst
-           (* Destruction *)
-           | [H: context [weq ?w1 ?w2] |- _] => destruct (weq w1 w2)
-           | [ |- context [weq ?w1 ?w2] ] => destruct (weq w1 w2)
-           end; dest; try subst; intuition idtac)
-      ).
+  Lemma procDec_inv_0_ok:
+    forall o,
+      reachable o (fst pdecInl) ->
+      procDec_inv_0 o.
+  Proof.
+    intros; inv H; inv H0.
+    eapply procDec_inv_0_ok'; eauto.
+  Qed.
 
   Lemma procDec_inv_1_ok':
     forall init n ll,
@@ -209,59 +263,26 @@ Section Invariants.
     eapply procDec_inv_1_ok'; eauto.
   Qed.
 
-  Lemma procDec_inv_0_ok':
+  Lemma procDec_inv_2_ok':
     forall init n ll,
       init = initRegs (getRegInits (fst pdecInl)) ->
       Multistep (fst pdecInl) init n ll ->
-      procDec_inv_0 n.
+      procDec_inv_2 n.
   Proof.
     admit.
-    (* induction 2. *)
-
-    (* - repeat subst. *)
-    (*   simpl; unfold procDec_inv_0. *)
-    (*   invReify; auto. *)
-
-    (* - specialize (IHMultistep H); clear -IHMultistep HStep. *)
-    (*   apply step_no_defs_substep in HStep; [|reflexivity]. *)
-    (*   destruct HStep as [ul [calls ?]]; dest; subst. *)
-    (*   inv H0; try (mred; fail); [|inv HIn]. *)
-    (*   CommonTactics.dest_in. *)
-
-    (*   + inv H; invertActionRep. *)
-    (*     unfold procDec_inv_0 in *; dest. *)
-    (*     invReify; simpl_find; auto. *)
-    (*   + inv H0; invertActionRep. *)
-    (*     unfold procDec_inv_0 in *; dest. *)
-    (*     invReify; simpl_find; auto. *)
-    (*   + inv H; invertActionRep. *)
-    (*     unfold procDec_inv_0 in *; dest. *)
-    (*     invReify; simpl_find; auto. *)
-    (*   + inv H0; invertActionRep. *)
-    (*     unfold procDec_inv_0 in *; dest. *)
-    (*     invReify; simpl_find; auto. *)
-    (*   + inv H; invertActionRep. *)
-    (*     unfold procDec_inv_0 in *; dest. *)
-    (*     invReify; simpl_find; auto. *)
-    (*   + inv H0; invertActionRep. *)
-    (*     unfold procDec_inv_0 in *; dest. *)
-    (*     invReify; simpl_find; auto. *)
-    (*   + inv H; invertActionRep. *)
-    (*     unfold procDec_inv_0 in *; dest. *)
-    (*     invReify; simpl_find; auto. *)
-    (*   + inv H0; invertActionRep. *)
-    (*     unfold procDec_inv_0 in *; dest. *)
-    (*     invReify; simpl_find; auto. *)
   Qed.
 
-  Lemma procDec_inv_0_ok:
+  Lemma procDec_inv_2_ok:
     forall o,
       reachable o (fst pdecInl) ->
-      procDec_inv_0 o.
+      procDec_inv_2 o.
   Proof.
     intros; inv H; inv H0.
-    eapply procDec_inv_0_ok'; eauto.
+    eapply procDec_inv_2_ok'; eauto.
   Qed.
 
 End Invariants.
+
+Hint Unfold xor3 procDec_inv_0 procDec_inv_1 procDec_inv_2
+     fifo_empty_inv fifo_not_empty_inv: InvDefs.
 
