examples/ProcDecInl.v
@@ -1,0 +1,33 @@
+Require Import Lts.Syntax Lts.Semantics Lts.Equiv Lts.Refinement Lts.Renaming Lts.Wf.
+Require Import Lts.Inline Lts.InlineFacts_2.
+Require Import Ex.SC Ex.ProcDec.
+
+Set Implicit Arguments.
+
+Section Inlined.
+  Variables addrSize fifoSize valSize rfIdx: nat.
+
+  Variable dec: DecT 2 addrSize valSize rfIdx.
+  Variable exec: ExecT 2 addrSize valSize rfIdx.
+
+  Definition pdec := pdecf fifoSize dec exec.
+  Hint Unfold pdec: ModuleDefs. (* for kinline_compute *)
+
+  Definition pdecInl: Modules * bool.
+  Proof.
+    remember (inlineF pdec) as inlined.
+    kinline_compute_in Heqinlined.
+    match goal with
+    | [H: inlined = ?m |- _] =>
+      exact m
+    end.
+  Defined.
+
+  Lemma pdecInl_equal: pdecInl = inlineF pdec.
+  Proof.
+    kinline_compute.
+    reflexivity.
+  Qed.
+
+End Inlined.
+
